WCCC/Proof/Conv.lean
@@ -1,0 +1,35 @@
+
+import Common
+import WCCC.Proof
+
+namespace WCCC.Conv
+
+  theorem refl : (CvTerm.refl t) : t === t := by {
+    induction t
+    all_goals try (simp; constructor <;> simp [*])
+  }
+
+  theorem subst : c : t === s -> ([▸σ]c) : [σ]t === [σ]s := by {
+    intro h
+    induction h generalizing σ <;> simp
+    case sym c t2 t1 h ih => constructor; apply ih
+    case trans c1 t1 t2 c2 t3 h1 h2 ih1 ih2 => constructor; apply ih1; apply ih2
+    case bound K x =>
+      unfold Term.subst_term_to_subst_cvterm <;> simp
+      cases (σ x) <;> simp
+      case _ => constructor
+      case _ => apply refl
+    case app_beta c b t t2 m A h ih =>
+      constructor; simp at *; apply ih
+    case all_congr c1 A1 A2 c2 B1 B2 m h1 h2 ih1 ih2 =>
+      replace ih2 := @ih2 ^σ; simp at ih2
+      constructor; apply ih1; apply ih2
+    case lam_eta c m A t1 t2 h ih =>
+      constructor; simp at *
+
+    case pair_erased c t1 t2 T1 s1 h ih =>
+      constructor; apply ih
+    repeat sorry
+  }
+
+end WCCC.Conv
